theories/sim/local.v
@@ -60,7 +60,7 @@ Inductive _sim_local_body_step (r_f : A) (sim_local_body : SIM)
              (* For any new resource r' that supports the returned values are
                 related w.r.t. (r ⋅ r' ⋅ r_f) *)
              (VRET: vrel r' (Val v_src) (Val v_tgt))
-             (* (STACK: σt'.(scs) = σt.(scs)) *),
+             (STACK: σt.(scs) = σt'.(scs)),
         ∃ idx', sim_local_body (rc ⋅ r') idx'
                                (fill Ks (Val v_src)) σs'
                                (fill Kt (Val v_tgt)) σt' Φ).
@@ -118,7 +118,7 @@ Proof.
     exists es', σs', r', idx'. do 2 (split; [done|]).
     pclearbot. right. eapply CIH; eauto.
   - econstructor 2; eauto. intros.
-    destruct (CONT _ _ _ σs' σt' VRET (* STACK *)) as [idx' SIM'].
+    destruct (CONT _ _ _ σs' σt' VRET STACK) as [idx' SIM'].
     exists idx'. pclearbot. right. eapply CIH; eauto.
 Qed.
 
